make only latest val visible in msv. leads to more simple proofs, and hopefully easier physical correspondence

src/program_proof/pav/core.v
@@ -1,11 +1,6 @@
 From Perennial.program_proof Require Import grove_prelude.
 From Perennial.program_proof.pav Require Import serde.
 
-(*
-From Perennial.base_logic.lib Require Import ghost_map.
-From iris.unstable.base_logic Require Import mono_list.
-*)
-
 From RecordUpdate Require Export RecordSet.
 From Perennial.base_logic.lib Require Export ghost_map.
 From iris.unstable.base_logic Require Export mono_list.
@@ -32,6 +27,7 @@ Notation merkle_map_ty := (gmap (list w8) (list w8)) (only parsing).
 Notation map_adtr_ty := (gmap opaque_label_ty (epoch_ty * comm_ty)) (only parsing).
 Notation cli_map_val_ty := (option (epoch_ty * comm_ty))%type (only parsing).
 Notation cli_map_ty := (gmap map_label_ty cli_map_val_ty) (only parsing).
+Notation lat_val_ty := (option (fake_ver_ty * fake_map_val_ty)) (only parsing).
 
 Section misc.
 Class pavG Σ :=
@@ -42,16 +38,15 @@ Class pavG Σ :=
   }.
 End misc.
 
-Section msv.
+Section msv_core.
 
 (* maximum sequence of versions. *)
 
-Definition msv_aux (m : fake_map_ty) uid vals :=
-  (* TODO: change to know elem exists there. *)
-  (∀ i, i < length vals → m !! (uid, i) = vals !! i).
+Definition msv_core_aux (m : fake_map_ty) uid (vals : list fake_map_val_ty) :=
+  (∀ ver val, vals !! ver = Some val → m !! (uid, ver) = Some val).
 
-Definition msv m uid vals :=
-  msv_aux m uid vals ∧
+Definition msv_core m uid vals :=
+  msv_core_aux m uid vals ∧
   m !! (uid, (length vals)) = None.
 
 (* TODO: upstream. *)
@@ -59,20 +54,19 @@ Lemma lookup_snoc {A} (l : list A) (x : A) :
   (l ++ [x]) !! (length l) = Some x.
 Proof. by opose proof (proj2 (lookup_snoc_Some x l (length l) x) _) as H; [naive_solver|]. Qed.
 
-Lemma msv_aux_snoc {m uid l x} :
-  msv_aux m uid (l ++ [x]) →
-  msv_aux m uid l ∧ m !! (uid, length l) = Some x.
+Lemma msv_core_aux_snoc {m uid l x} :
+  msv_core_aux m uid (l ++ [x]) →
+  msv_core_aux m uid l ∧ m !! (uid, length l) = Some x.
 Proof.
   intros HM. split.
-  - intros i ?. ospecialize (HM i _). { rewrite length_app/=. lia. }
-    by rewrite lookup_app_l in HM; [|lia].
-  - ospecialize (HM (length l) _). { rewrite length_app/=. lia. }
-    by rewrite lookup_snoc in HM.
+  - intros ?? Hlook. ospecialize (HM _ _ _); [|done].
+    rewrite lookup_app_l; [exact Hlook|by eapply lookup_lt_Some].
+  - ospecialize (HM (length l) _ _); [apply lookup_snoc|done].
 Qed.
 
-Lemma msv_aux_agree {m uid vals0 vals1} :
-  msv_aux m uid vals0 →
-  msv_aux m uid vals1 →
+Lemma msv_core_aux_agree {m uid vals0 vals1} :
+  msv_core_aux m uid vals0 →
+  msv_core_aux m uid vals1 →
   length vals0 = length vals1 →
   vals0 = vals1.
 Proof.
@@ -82,44 +76,65 @@ Proof.
   - rewrite length_app/=. lia.
   - rewrite length_app/=. lia.
   - rewrite !length_app/=. intros H0 H1 ?.
-    apply msv_aux_snoc in H0 as [H0 Hx0]. apply msv_aux_snoc in H1 as [H1 Hx1].
+    apply msv_core_aux_snoc in H0 as [H0 Hx0]. apply msv_core_aux_snoc in H1 as [H1 Hx1].
     assert (length l0 = length l1) as HT by lia. rewrite HT in Hx0. clear HT.
     simplify_map_eq/=. ospecialize (IH l1 _ _ _); [done..|lia|]. naive_solver.
 Qed.
 
-Lemma msv_len_agree_aux {m uid vals0 vals1} :
-  msv m uid vals0 →
-  msv m uid vals1 →
+Lemma msv_core_len_agree_aux {m uid vals0 vals1} :
+  msv_core m uid vals0 →
+  msv_core m uid vals1 →
   length vals0 < length vals1 →
   False.
 Proof.
-  intros HM0 HM1 ?. destruct HM0 as [_ HM0]. destruct HM1 as [HM1 _].
-  ospecialize (HM1 (length vals0) _); [lia|].
-  opose proof (lookup_lt_is_Some_2 vals1 (length vals0) _) as [? Hsome]; [lia|].
-  rewrite Hsome in HM1. naive_solver.
+  intros HM0 HM1 ?. destruct HM0 as [_ HM0], HM1 as [HM1 _].
+  list_elem vals1 (length vals0) as val.
+  ospecialize (HM1 _ _ _); [exact Hval_lookup|naive_solver].
 Qed.
 
-Lemma msv_len_agree {m uid vals0 vals1} :
-  msv m uid vals0 →
-  msv m uid vals1 →
+Lemma msv_core_len_agree {m uid vals0 vals1} :
+  msv_core m uid vals0 →
+  msv_core m uid vals1 →
   length vals0 = length vals1.
 Proof.
-  intros ??.
+  intros Hcore0 Hcore1.
   destruct (decide (length vals0 = length vals1)) as [?|?]; [done|].
   exfalso. destruct (decide (length vals0 < length vals1)) as [?|?].
-  - eapply (msv_len_agree_aux (vals0:=vals0) (vals1:=vals1)); [done..|lia].
-  - eapply (msv_len_agree_aux (vals0:=vals1) (vals1:=vals0)); [done..|lia].
+  - eapply (msv_core_len_agree_aux Hcore0 Hcore1); [done..|lia].
+  - eapply (msv_core_len_agree_aux Hcore1 Hcore0); [done..|lia].
 Qed.
 
-Lemma msv_agree {m uid vals0 vals1} :
-  msv m uid vals0 →
-  msv m uid vals1 →
+Lemma msv_core_agree {m uid vals0 vals1} :
+  msv_core m uid vals0 →
+  msv_core m uid vals1 →
   vals0 = vals1.
 Proof.
-  intros HM0 HM1. eapply msv_aux_agree.
+  intros HM0 HM1. eapply msv_core_aux_agree.
   - by destruct HM0 as [? _].
   - by destruct HM1 as [? _].
-  - by eapply msv_len_agree.
+  - by eapply msv_core_len_agree.
+Qed.
+
+End msv_core.
+
+Section msv.
+
+(* msv hides all but the latest val.
+a None val corresponds to an unregistered val. *)
+Definition msv (m : fake_map_ty) uid (lat : lat_val_ty) :=
+  let len_vals := match lat with None => 0 | Some (ver, val) => S ver end in
+  ∃ vals, length vals = len_vals ∧ last vals = snd <$> lat ∧
+  msv_core m uid vals.
+
+Lemma msv_agree {m uid val0 val1} :
+  msv m uid val0 →
+  msv m uid val1 →
+  val0 = val1.
+Proof.
+  intros HM0 HM1.
+  destruct HM0 as (?&Hlen0&?&HM0). destruct HM1 as (?&Hlen1&?&HM1).
+  pose proof (msv_core_agree HM0 HM1) as ->. rewrite Hlen0 in Hlen1.
+  destruct val0 as [[??]|], val1 as [[??]|]; naive_solver.
 Qed.
 
 End msv.
@@ -127,6 +142,53 @@ End msv.
 Section hist_msv.
 
 (* history and its interaction with msv. *)
+
+(* TODO: took out adtr epoch check. do i still need it? *)
+Definition adtr_inv' (ms : list fake_map_ty) :=
+  ∀ i j mi mj,
+  ms !! i = Some mi →
+  ms !! j = Some mj →
+  i ≤ j →
+  mi ⊆ mj.
+
+Definition know_hist_val (ms : list fake_map_ty) (uid : w64) (ep : nat) (lat : lat_val_ty) :=
+  let len_vals := match lat with None => 0 | Some (ver, val) => S ver end in
+  (* TODO: this is one way to write it. consolidates cases.
+  let's see how easy it is to prove with the physical hist. *)
+  ∃ vals, length vals = len_vals ∧ last vals = snd <$> lat ∧
+  (* vals exist in prior maps. *)
+  (∀ ver val, vals !! ver = Some val →
+    (∃ prior m, prior ≤ ep ∧ ms !! prior = Some m ∧ m !! (uid, ver) = Some val)) ∧
+  (* next ver doesn't exist in some future map. *)
+  (∃ bound m, bound ≥ ep ∧ ms !! bound = Some m ∧ m !! (uid, length vals) = None).
+
+Definition know_hist (ms : list fake_map_ty) (uid : w64) (hist : list lat_val_ty) :=
+  (∀ ep lat, hist !! ep = Some lat → know_hist_val ms uid ep lat).
+
+(* hist_msv says that for every latest val in the hist,
+we can derive an msv for it. *)
+Lemma hist_msv ms uid hist ep m lat :
+  adtr_inv' ms →
+  know_hist ms uid hist →
+  hist !! ep = Some lat →
+  ms !! ep = Some m →
+  msv m uid lat.
+Proof.
+  intros Hadtr Hhist Hlook_entry Hlook_m.
+  specialize (Hhist _ _ Hlook_entry) as (vals&?&?&Hhist&Hbound).
+  exists vals. split_and?; [done..|split].
+  - intros ?? Hlook_ver.
+    specialize (Hhist _ _ Hlook_ver) as (?&?&?&?Hlook_prior&?).
+    opose proof (Hadtr _ _ _ _ Hlook_prior Hlook_m _); [lia|].
+    by eapply lookup_weaken.
+  - destruct Hbound as (?&?&?&Hlook_bound&?).
+    opose proof (Hadtr _ _ _ _ Hlook_m Hlook_bound _); [lia|].
+    by eapply lookup_weaken_None.
+Qed.
+
+End hist_msv.
+
+Section proper_adtr_inv.
 
 Definition lower_adtr (m : map_adtr_ty) : merkle_map_ty :=
   (λ v, MapValPre.encodesF (MapValPre.mk v.1 v.2)) <$> m.
@@ -150,60 +212,4 @@ Definition maps_epoch_ok (ms : list map_adtr_ty) :=
 
 Definition adtr_inv ms := maps_mono (lower_adtr <$> ms) ∧ maps_epoch_ok ms.
 
-(* tmp duplicate adtr invs that use the same map type as below. *)
-Definition maps_mono' (ms : list fake_map_ty) :=
-  ∀ i j mi mj,
-  ms !! i = Some mi →
-  ms !! j = Some mj →
-  i ≤ j →
-  mi ⊆ mj.
-
-Definition maps_epoch_ok' (ms : list fake_map_ty) :=
-  ∃ ep m_ep uid ver ep' val,
-  ms !! ep = Some m_ep →
-  m_ep !! (uid, ver) = Some (ep', val) →
-  ep' ≤ ep.
-
-Definition adtr_inv' ms := maps_mono' ms ∧ maps_epoch_ok' ms.
-
-Record hist_entry_ty :=
-  mk_hist_entry {
-    (* TODO: make msv only talk about latest val at some version.
-    this seems to more naturally capture what people care abt with KT.
-    and it'd allow us to only make visible the latest val and version here.
-    do this by proving new msv on top of old one. *)
-    vals: list (nat * list w8);
-  }.
-
-Definition know_entry (uid : w64) (ep : nat) (entry : hist_entry_ty) (ms : list fake_map_ty) :=
-  (* vals exist in prior maps. *)
-  (∀ ver val, entry.(vals) !! ver = Some val →
-    (∃ prior m, prior ≤ ep ∧ ms !! prior = Some m ∧ m !! (uid, ver) = Some val)) ∧
-  (* next ver doesn't exist in some future map. *)
-  (∃ bound m, bound ≥ ep ∧ ms !! bound = Some m ∧ m !! (uid, length entry.(vals)) = None).
-
-Definition know_hist (uid : w64) (hist : list hist_entry_ty) (ms : list fake_map_ty) :=
-  (∀ ep entry, hist !! ep = Some entry → know_entry uid ep entry ms).
-
-Lemma hist_msv ms uid hist ep m entry :
-  adtr_inv' ms →
-  know_hist uid hist ms →
-  hist !! ep = Some entry →
-  ms !! ep = Some m →
-  msv m uid entry.(vals).
-Proof.
-  intros Hadtr Hhist Hlook_entry Hlook_m. split.
-  - intros ver Hlook_ver.
-    specialize (Hhist _ _ Hlook_entry) as [Hhist _].
-    list_elem entry.(vals) ver as val.
-    specialize (Hhist _ _ Hval_lookup) as (?&?&?&Hlook_prior&Hlook_mprior).
-    opose proof ((proj1 Hadtr) _ _ _ _ Hlook_prior Hlook_m _); [lia|].
-    rewrite Hval_lookup.
-    by eapply lookup_weaken.
-  - specialize (Hhist _ _ Hlook_entry).
-    destruct Hhist as [_ (bound&mbound&Hlt_bound&Hlook_bound&Hlook_mbound)].
-    opose proof ((proj1 Hadtr) _ _ _ _ Hlook_m Hlook_bound _); [lia|].
-    by eapply lookup_weaken_None.
-Qed.
-
-End hist_msv.
+End proper_adtr_inv.
